rename emp, star, valid_synth according to the paper

tests/layeff/LowParseWriters.Compat.fst
@@ -5,9 +5,9 @@ friend LowParseWriters.Parsers
 
 module B = LowStar.Buffer
 
-let emp_correct = ()
+let parse_empty_correct = ()
 
-let star_correct
+let parse_pair_correct
   p1 p2
 = ()
 
@@ -18,26 +18,26 @@ let parse_synth
     (LP.serialize_synth (Parser?.p p1).parser f2 (Parser?.p p1).serializer f1 ())
     (LP.jump_synth (Parser?.p p1).jumper f2 ())
 
-let valid_synth_parse_synth
+let valid_rewrite_parse_synth
   p1 #t2 f2 f1 sq
 = {
-  valid_synth_valid = (fun h b pos pos' ->
+  valid_rewrite_valid = (fun h b pos pos' ->
     LP.valid_synth h (get_parser p1) f2 (LP.make_slice b (B.len b)) pos
   );
-  valid_synth_size = (fun x ->
+  valid_rewrite_size = (fun x ->
     LP.synth_injective_synth_inverse_synth_inverse_recip f2 f1 ();
     LP.serialize_synth_eq (get_parser p1) f2 (Parser?.p p1).serializer f1 () (f2 x)
   );
 }
 
-let valid_synth_parse_synth_recip
+let valid_rewrite_parse_synth_recip
   p1 #t2 f2 f1 sq
 = {
-  valid_synth_valid = (fun h b pos pos' ->
+  valid_rewrite_valid = (fun h b pos pos' ->
     LP.synth_injective_synth_inverse_synth_inverse_recip f2 f1 ();
     LP.valid_synth h (get_parser p1) f2 (LP.make_slice b (B.len b)) pos
   );
-  valid_synth_size = (fun x ->
+  valid_rewrite_size = (fun x ->
     LP.serialize_synth_eq (get_parser p1) f2 (Parser?.p p1).serializer f1 () (x)
   );
 }
@@ -66,10 +66,10 @@ let parse_enum
     (LP.serialize_enum_key _ (get_serializer p) e)
     (LP.jump_enum_key (Parser?.p p).jumper e)
 
-let valid_synth_parse_sum
+let valid_rewrite_parse_sum
   ps pe p k pk
 = {
-  valid_synth_valid = (fun h b pos pos' ->
+  valid_rewrite_valid = (fun h b pos pos' ->
     let sl = LP.make_slice b (B.len b) in
     assert (LP.valid (LP.parse_enum_key ps.sum_p (LP.sum_enum ps.sum_t) `LP.nondep_then` dsnd (ps.sum_pc k)) h sl pos);
     let (k', _) = LP.contents (LP.parse_enum_key ps.sum_p (LP.sum_enum ps.sum_t) `LP.nondep_then` dsnd (ps.sum_pc k)) h sl pos in
@@ -79,8 +79,8 @@ let valid_synth_parse_sum
     assert (LP.contents (LP.parse_enum_key ps.sum_p (LP.sum_enum ps.sum_t)) h sl pos == k);
     LP.valid_sum_intro h ps.sum_t ps.sum_p ps.sum_pc sl pos
   );
-  valid_synth_size = (fun x ->
-    let (k', pl) = LP.coerce (Parser?.t pe & Parser?.t pk) (x <: (Parser?.t (pe `star` pk))) in
+  valid_rewrite_size = (fun x ->
+    let (k', pl) = LP.coerce (Parser?.t pe & Parser?.t pk) (x <: (Parser?.t (pe `parse_pair` pk))) in
     let y = LP.synth_sum_case ps.sum_t k pl in
     assert (LP.sum_tag_of_data ps.sum_t y == k);
     LP.synth_sum_case_inverse ps.sum_t k;
@@ -99,10 +99,10 @@ let parse_maybe_enum
     (LP.serialize_maybe_enum_key _ (get_serializer p) e)
     (LP.jump_maybe_enum_key (Parser?.p p).jumper e)
 
-let valid_synth_parse_dsum_known
+let valid_rewrite_parse_dsum_known
   ps pe p k pk
 = {
-  valid_synth_valid = (fun h b pos pos' ->
+  valid_rewrite_valid = (fun h b pos pos' ->
     let sl = LP.make_slice b (B.len b) in
     assert (LP.valid (LP.parse_maybe_enum_key ps.dsum_p (LP.dsum_enum ps.dsum_t) `LP.nondep_then` dsnd (ps.dsum_pc k)) h sl pos);
     let (k', _) = LP.contents (LP.parse_maybe_enum_key ps.dsum_p (LP.dsum_enum ps.dsum_t) `LP.nondep_then` dsnd (ps.dsum_pc k)) h sl pos in
@@ -112,8 +112,8 @@ let valid_synth_parse_dsum_known
     assert (LP.contents (LP.parse_maybe_enum_key ps.dsum_p (LP.dsum_enum ps.dsum_t)) h sl pos == LP.Known k);
     LP.valid_dsum_intro_known h ps.dsum_t ps.dsum_p ps.dsum_pc ps.dsum_pu sl pos
   );
-  valid_synth_size = (fun x ->
-    let (k', pl) = LP.coerce (Parser?.t pe & Parser?.t pk) (x <: (Parser?.t (pe `star` pk))) in
+  valid_rewrite_size = (fun x ->
+    let (k', pl) = LP.coerce (Parser?.t pe & Parser?.t pk) (x <: (Parser?.t (pe `parse_pair` pk))) in
     let y = LP.synth_dsum_case ps.dsum_t (LP.Known k) pl in
     assert (LP.dsum_tag_of_data ps.dsum_t y == LP.Known k);
     LP.synth_dsum_case_inverse ps.dsum_t (LP.Known k);
@@ -124,10 +124,10 @@ let valid_synth_parse_dsum_known
   );
 }
 
-let valid_synth_parse_dsum_unknown
+let valid_rewrite_parse_dsum_unknown
   ps pe p pu
 = {
-  valid_synth_valid = (fun h b pos pos' ->
+  valid_rewrite_valid = (fun h b pos pos' ->
     let sl = LP.make_slice b (B.len b) in
     assert (LP.valid (LP.parse_maybe_enum_key ps.dsum_p (LP.dsum_enum ps.dsum_t) `LP.nondep_then` (ps.dsum_pu)) h sl pos);
     let (k', _) = LP.contents (LP.parse_maybe_enum_key ps.dsum_p (LP.dsum_enum ps.dsum_t) `LP.nondep_then` (ps.dsum_pu)) h sl pos in
@@ -137,8 +137,8 @@ let valid_synth_parse_dsum_unknown
     assert (LP.Unknown? (LP.contents (LP.parse_maybe_enum_key ps.dsum_p (LP.dsum_enum ps.dsum_t)) h sl pos));
     LP.valid_dsum_intro_unknown h ps.dsum_t ps.dsum_p ps.dsum_pc ps.dsum_pu sl pos
   );
-  valid_synth_size = (fun x ->
-    let (k', pl) = LP.coerce (Parser?.t pe & Parser?.t pu) (x <: (Parser?.t (pe `star` pu))) in
+  valid_rewrite_size = (fun x ->
+    let (k', pl) = LP.coerce (Parser?.t pe & Parser?.t pu) (x <: (Parser?.t (pe `parse_pair` pu))) in
     let y = LP.synth_dsum_case ps.dsum_t (k') pl in
     assert (LP.dsum_tag_of_data ps.dsum_t y == k');
     LP.synth_dsum_case_inverse ps.dsum_t (k');
@@ -149,38 +149,38 @@ let valid_synth_parse_dsum_unknown
   );
 }
 
-let valid_synth_parse_vlarray_intro
+let valid_rewrite_parse_vlarray_intro
   pa p array_byte_size_min array_byte_size_max elem_count_min elem_count_max u
 =
   LP.vldata_to_vlarray_inj (U32.v array_byte_size_min) (U32.v array_byte_size_max) (get_serializer p) elem_count_min elem_count_max u;
   LP.vlarray_to_vldata_to_vlarray (U32.v array_byte_size_min) (U32.v array_byte_size_max) (get_serializer p) elem_count_min elem_count_max u;
-  valid_synth_implies
+  valid_rewrite_implies
     _ _ _ _
-    (valid_synth_compose
+    (valid_rewrite_compose
       _ _ _ _
-      (valid_synth_parse_synth
+      (valid_rewrite_parse_synth
         (parse_vllist p array_byte_size_min array_byte_size_max)
         (LP.vldata_to_vlarray (U32.v array_byte_size_min) (U32.v array_byte_size_max) (get_serializer p) elem_count_min elem_count_max u)
         (LP.vlarray_to_vldata (U32.v array_byte_size_min) (U32.v array_byte_size_max) (get_serializer p) elem_count_min elem_count_max u)
         ()
       )
       _ _ _
-      (valid_synth_parser_eq _ _)
+      (valid_rewrite_parser_eq _ _)
     )
     _ _
 
-let valid_synth_parse_vlarray_elim
+let valid_rewrite_parse_vlarray_elim
   pa p array_byte_size_min array_byte_size_max elem_count_min elem_count_max u
 =
   LP.vldata_to_vlarray_inj (U32.v array_byte_size_min) (U32.v array_byte_size_max) (get_serializer p) elem_count_min elem_count_max u;
   LP.vlarray_to_vldata_to_vlarray (U32.v array_byte_size_min) (U32.v array_byte_size_max) (get_serializer p) elem_count_min elem_count_max u;
-  valid_synth_implies
+  valid_rewrite_implies
     _ _ _ _
-    (valid_synth_compose
+    (valid_rewrite_compose
       _ _ _ _
-      (valid_synth_parser_eq _ _)
+      (valid_rewrite_parser_eq _ _)
       _ _ _
-      (valid_synth_parse_synth_recip
+      (valid_rewrite_parse_synth_recip
         (parse_vllist p array_byte_size_min array_byte_size_max)
         (LP.vldata_to_vlarray (U32.v array_byte_size_min) (U32.v array_byte_size_max) (get_serializer p) elem_count_min elem_count_max u)
         (LP.vlarray_to_vldata (U32.v array_byte_size_min) (U32.v array_byte_size_max) (get_serializer p) elem_count_min elem_count_max u)
@@ -189,17 +189,16 @@ let valid_synth_parse_vlarray_elim
     )
     _ _
 
-let valid_synth_parse_bounded_vldata_intro
+let valid_rewrite_parse_bounded_vldata_intro
   pa p min max
 = {
-  valid_synth_valid = (fun h b pos pos' ->
+  valid_rewrite_valid = (fun h b pos pos' ->
     assert (valid_pos (parse_vldata p min max) h b pos pos');
     let sl = LP.make_slice b (B.len b) in
     LP.valid_bounded_vldata_strong_elim h (U32.v min) (U32.v max) (get_serializer p) sl pos;
     LP.valid_bounded_vldata_intro h (U32.v min) (U32.v max) (get_parser p) sl pos pos'
   );
-  valid_synth_size = (fun (x: Parser?.t (parse_vldata p min max)) ->
+  valid_rewrite_size = (fun (x: Parser?.t (parse_vldata p min max)) ->
     LP.serializer_unique (get_parser pa) (get_serializer pa) (LP.serialize_bounded_vldata (U32.v min) (U32.v max) (get_serializer p)) x
   );
 }
-  
