tests/layeff/LowParseWriters.Sealed.Compat.fst
@@ -4,7 +4,7 @@ include LowParseWriters.Sealed
 
 module LP = LowParse.Low
 
-let valid_synth_parse_synth'
+let valid_rewrite_parse_synth'
   (p1: parser)
   (#t2: Type)
   (f2: Parser?.t p1 -> GTot t2)
@@ -13,10 +13,10 @@ let valid_synth_parse_synth'
     LP.synth_injective f2 /\
     LP.synth_inverse f2 f1
   ))
-: Tot (squash (valid_synth_prop p1 (parse_synth p1 f2 f1)))
-= tvalid_synth_of_evalid_synth (valid_synth_parse_synth p1 f2 f1 sq)
+: Tot (squash (valid_rewrite_prop p1 (parse_synth p1 f2 f1)))
+= tvalid_rewrite_of_evalid_rewrite (valid_rewrite_parse_synth p1 f2 f1 sq)
 
-let valid_synth_parse_synth_recip'
+let valid_rewrite_parse_synth_recip'
   (p1: parser)
   (#t2: Type)
   (f2: Parser?.t p1 -> GTot t2)
@@ -25,12 +25,12 @@ let valid_synth_parse_synth_recip'
     LP.synth_injective f2 /\
     LP.synth_inverse f2 f1
   ))
-: Tot (squash (valid_synth_prop (parse_synth p1 f2 f1) p1))
-= tvalid_synth_of_evalid_synth (valid_synth_parse_synth_recip p1 f2 f1 sq)
+: Tot (squash (valid_rewrite_prop (parse_synth p1 f2 f1) p1))
+= tvalid_rewrite_of_evalid_rewrite (valid_rewrite_parse_synth_recip p1 f2 f1 sq)
 
 module U32 = FStar.UInt32
 
-let valid_synth_parse_vlarray_intro'
+let valid_rewrite_parse_vlarray_intro'
   (pa: parser)
   (p: parser1)
   (array_byte_size_min: U32.t)
@@ -43,14 +43,14 @@ let valid_synth_parse_vlarray_intro'
     Parser?.t pa == LP.vlarray (Parser?.t p) elem_count_min elem_count_max /\
     get_parser pa == LP.parse_vlarray (U32.v array_byte_size_min) (U32.v array_byte_size_max) (get_serializer p) elem_count_min elem_count_max ()
   ))
-: Tot (squash (valid_synth_prop
+: Tot (squash (valid_rewrite_prop
     (parse_vllist p array_byte_size_min array_byte_size_max)
     pa
   ))
 =
-  tvalid_synth_of_evalid_synth (valid_synth_parse_vlarray_intro pa p array_byte_size_min array_byte_size_max elem_count_min elem_count_max u)
+  tvalid_rewrite_of_evalid_rewrite (valid_rewrite_parse_vlarray_intro pa p array_byte_size_min array_byte_size_max elem_count_min elem_count_max u)
 
-let valid_synth_parse_vlarray_elim'
+let valid_rewrite_parse_vlarray_elim'
   (pa: parser)
   (p: parser1)
   (array_byte_size_min: U32.t)
@@ -63,14 +63,14 @@ let valid_synth_parse_vlarray_elim'
     Parser?.t pa == LP.vlarray (Parser?.t p) elem_count_min elem_count_max /\
     get_parser pa == LP.parse_vlarray (U32.v array_byte_size_min) (U32.v array_byte_size_max) (get_serializer p) elem_count_min elem_count_max ()
   ))
-: Tot (squash (valid_synth_prop
+: Tot (squash (valid_rewrite_prop
     pa
     (parse_vllist p array_byte_size_min array_byte_size_max)
   ))
 =
-  tvalid_synth_of_evalid_synth (valid_synth_parse_vlarray_elim pa p array_byte_size_min array_byte_size_max elem_count_min elem_count_max u)
+  tvalid_rewrite_of_evalid_rewrite (valid_rewrite_parse_vlarray_elim pa p array_byte_size_min array_byte_size_max elem_count_min elem_count_max u)
 
-let valid_synth_parse_bounded_vldata_intro'
+let valid_rewrite_parse_bounded_vldata_intro'
   (pa: parser)
   (p: parser)
   (min: U32.t)
@@ -82,12 +82,12 @@ let valid_synth_parse_bounded_vldata_intro'
     get_parser_kind pa == LP.parse_bounded_vldata_strong_kind (U32.v min) (U32.v max) (LP.log256' (U32.v max)) (get_parser_kind p) /\
     get_parser pa == LP.parse_bounded_vldata (U32.v min) (U32.v max) (get_parser p)
   })
-: Tot (squash (valid_synth_prop
+: Tot (squash (valid_rewrite_prop
     (parse_vldata p min max)
     pa
   ))
 =
-  tvalid_synth_of_evalid_synth (valid_synth_parse_bounded_vldata_intro pa p min max)
+  tvalid_rewrite_of_evalid_rewrite (valid_rewrite_parse_bounded_vldata_intro pa p min max)
 
 inline_for_extraction
 noextract
@@ -104,8 +104,8 @@ let parse_bounded_vldata_intro_ho'
     get_parser_kind pa == LP.parse_bounded_vldata_strong_kind (U32.v min) (U32.v max) (LP.log256' (U32.v max)) (get_parser_kind p) /\
     get_parser pa == LP.parse_bounded_vldata (U32.v min) (U32.v max) (get_parser p)
   })
-  (f: (unit -> TWrite unit emp p inv))
-: TWrite unit emp pa
+  (f: (unit -> TWrite unit parse_empty p inv))
+: TWrite unit parse_empty pa
     inv
 =
   twrite_of_ewrite (fun _ -> parse_bounded_vldata_intro_ho' pa p min max (fun _ -> ewrite_of_twrite f))
